Parameters are not needed anymore, contd

ConsensusSafety.thy
@@ -14,20 +14,20 @@ fun (in Protocol) futures :: "state \<Rightarrow> state set"
 
 (* Lemma 1 *)
 lemma (in Protocol) monotonic_futures :
-  "\<forall> \<sigma>' \<sigma>. is_valid_params \<and> \<sigma>' \<in> \<Sigma>t \<and> \<sigma> \<in> \<Sigma>t
+  "\<forall> \<sigma>' \<sigma>. \<sigma>' \<in> \<Sigma>t \<and> \<sigma> \<in> \<Sigma>t
    \<longrightarrow> \<sigma>' \<in> futures \<sigma> \<longleftrightarrow> futures \<sigma>' \<subseteq> futures \<sigma>"
   by auto
 
 (* Theorem 1 *)
 theorem (in Protocol) two_party_common_futures :
-  "\<forall> \<sigma>1 \<sigma>2. is_valid_params \<and> \<sigma>1 \<in> \<Sigma>t \<and> \<sigma>2 \<in> \<Sigma>t
+  "\<forall> \<sigma>1 \<sigma>2. \<sigma>1 \<in> \<Sigma>t \<and> \<sigma>2 \<in> \<Sigma>t
   \<longrightarrow> (\<sigma>1 \<union> \<sigma>2) \<in> \<Sigma>t
   \<longrightarrow> futures \<sigma>1 \<inter> futures \<sigma>2 \<noteq> \<emptyset>"
   by auto
 
 (* Theorem 2 *)
 theorem (in Protocol) n_party_common_futures :
-  "\<forall> \<sigma>_set. is_valid_params \<and> \<sigma>_set \<subseteq> \<Sigma>t
+  "\<forall> \<sigma>_set. \<sigma>_set \<subseteq> \<Sigma>t
   \<longrightarrow> \<Union> \<sigma>_set \<in> \<Sigma>t
   \<longrightarrow> \<Inter> {futures \<sigma> | \<sigma>. \<sigma> \<in> \<sigma>_set} \<noteq> \<emptyset>"
   by auto
@@ -49,7 +49,7 @@ fun (in Protocol) state_property_is_decided :: "(state_property * state) \<Right
 
 (* Lemma 2 *)
 lemma (in Protocol) forward_consistency :
-  "\<forall> \<sigma>' \<sigma>. is_valid_params \<and> \<sigma>' \<in> \<Sigma>t \<and> \<sigma> \<in> \<Sigma>t
+  "\<forall> \<sigma>' \<sigma>. \<sigma>' \<in> \<Sigma>t \<and> \<sigma> \<in> \<Sigma>t
   \<longrightarrow> \<sigma>' \<in> futures \<sigma> 
   \<longrightarrow> state_property_is_decided (p, \<sigma>)
   \<longrightarrow> state_property_is_decided (p, \<sigma>')"
@@ -58,7 +58,7 @@ lemma (in Protocol) forward_consistency :
 
 (* Lemma 3 *)
 lemma (in Protocol) backword_consistency :
-  "\<forall> \<sigma>' \<sigma>. is_valid_params \<and> \<sigma>' \<in> \<Sigma>t \<and> \<sigma> \<in> \<Sigma>t
+  "\<forall> \<sigma>' \<sigma>. \<sigma>' \<in> \<Sigma>t \<and> \<sigma> \<in> \<Sigma>t
   \<longrightarrow> \<sigma>' \<in> futures \<sigma> 
   \<longrightarrow> state_property_is_decided (p, \<sigma>')
   \<longrightarrow> \<not>state_property_is_decided (state_property_not p, \<sigma>)"
@@ -67,7 +67,7 @@ lemma (in Protocol) backword_consistency :
   
 (* Theorem 3 *)
 theorem (in Protocol) two_party_consensus_safety :
-  "\<forall> \<sigma>1 \<sigma>2. is_valid_params \<and> \<sigma>1 \<in> \<Sigma>t \<and> \<sigma>2 \<in> \<Sigma>t
+  "\<forall> \<sigma>1 \<sigma>2. \<sigma>1 \<in> \<Sigma>t \<and> \<sigma>2 \<in> \<Sigma>t
   \<longrightarrow> (\<sigma>1 \<union> \<sigma>2) \<in> \<Sigma>t
   \<longrightarrow> \<not>(state_property_is_decided (p, \<sigma>1) \<and> state_property_is_decided (state_property_not p, \<sigma>2))"
   by auto
@@ -75,12 +75,12 @@ theorem (in Protocol) two_party_consensus_safety :
 (* Definition 3.4 *)
 fun (in Protocol) state_properties_are_inconsistent :: "state_property set \<Rightarrow> bool"
   where
-    "state_properties_are_inconsistent p_set = (\<forall> \<sigma> \<in> \<Sigma> protocol. \<not> (\<forall> p \<in> p_set. p \<sigma>))"
+    "state_properties_are_inconsistent p_set = (\<forall> \<sigma> \<in> \<Sigma>. \<not> (\<forall> p \<in> p_set. p \<sigma>))"
 
 (* Definition 3.5 *)
 fun (in Protocol) state_properties_are_consistent :: "state_property set \<Rightarrow> bool"
   where
-    "state_properties_are_consistent p_set = (\<exists> \<sigma> \<in> \<Sigma> protocol. \<forall> p \<in> p_set. p \<sigma>)"
+    "state_properties_are_consistent p_set = (\<exists> \<sigma> \<in> \<Sigma>. \<forall> p \<in> p_set. p \<sigma>)"
 
 (* Definition 3.6 *)
 fun (in Protocol) state_property_decisions :: "state \<Rightarrow> state_property set"
@@ -100,48 +100,45 @@ type_synonym consensus_value_property = "consensus_value \<Rightarrow> bool"
 (* Definition 3.8 *)
 fun (in Protocol) naturally_corresponding_state_property :: "consensus_value_property \<Rightarrow> state_property"
   where 
-    "naturally_corresponding_state_property q = (\<lambda>\<sigma>. \<forall> c \<in> \<epsilon> params \<sigma>. q c)"
+    "naturally_corresponding_state_property q = (\<lambda>\<sigma>. \<forall> c \<in> \<epsilon> \<sigma>. q c)"
 
 (* Definition 3.9 *)
 fun (in Protocol) consensus_value_properties_are_consistent :: "consensus_value_property set \<Rightarrow> bool"
   where
-    "consensus_value_properties_are_consistent q_set = (\<exists> c \<in> C params. \<forall> q \<in> q_set. q c)"
+    "consensus_value_properties_are_consistent q_set = (\<exists> c \<in> C. \<forall> q \<in> q_set. q c)"
 
 (* Lemma 4 *)
 lemma (in Protocol) naturally_corresponding_consistency :
-  "\<forall> q_set. is_valid_params
-  \<longrightarrow> state_properties_are_consistent {naturally_corresponding_state_property q | q. q \<in> q_set}
+  "\<forall> q_set. state_properties_are_consistent {naturally_corresponding_state_property q | q. q \<in> q_set}
   \<longrightarrow> consensus_value_properties_are_consistent q_set"
-  apply (rule, rule, rule)
+  apply (rule, rule)
 proof -
   fix q_set
-  assume hyp: "is_valid_params"
 
   have 
     "state_properties_are_consistent {naturally_corresponding_state_property q | q. q \<in> q_set}
-    \<longrightarrow> (\<exists> \<sigma> \<in> \<Sigma> protocol. \<forall> p \<in> {\<lambda>\<sigma>'. \<forall> c \<in> \<epsilon> params \<sigma>'. q c | q. q \<in> q_set}. p \<sigma>)"
+    \<longrightarrow> (\<exists> \<sigma> \<in> \<Sigma>. \<forall> p \<in> {\<lambda>\<sigma>'. \<forall> c \<in> \<epsilon> \<sigma>'. q c | q. q \<in> q_set}. p \<sigma>)"
     by simp
   moreover have
-    "(\<exists> \<sigma> \<in> \<Sigma> protocol. \<forall> p \<in> {\<lambda>\<sigma>'. \<forall> c \<in> \<epsilon> params \<sigma>'. q c | q. q \<in> q_set}. p \<sigma>)
-    \<longrightarrow> (\<exists> \<sigma> \<in> \<Sigma> protocol. \<forall> q' \<in> q_set. (\<lambda>\<sigma>'. \<forall> c \<in> \<epsilon> params \<sigma>'. q' c) \<sigma>)"
+    "(\<exists> \<sigma> \<in> \<Sigma>. \<forall> p \<in> {\<lambda>\<sigma>'. \<forall> c \<in> \<epsilon> \<sigma>'. q c | q. q \<in> q_set}. p \<sigma>)
+    \<longrightarrow> (\<exists> \<sigma> \<in> \<Sigma>. \<forall> q' \<in> q_set. (\<lambda>\<sigma>'. \<forall> c \<in> \<epsilon> \<sigma>'. q' c) \<sigma>)"
     by (metis (mono_tags, lifting) mem_Collect_eq)
   moreover have
-    "(\<exists> \<sigma> \<in> \<Sigma> protocol. \<forall> q \<in> q_set. (\<lambda>\<sigma>'. \<forall> c \<in> \<epsilon> params \<sigma>'. q c) \<sigma>)
-    \<longrightarrow> (\<exists> \<sigma> \<in> \<Sigma> protocol. \<forall> q' \<in> q_set. \<forall> c \<in> \<epsilon> params \<sigma>. q' c)"
+    "(\<exists> \<sigma> \<in> \<Sigma>. \<forall> q \<in> q_set. (\<lambda>\<sigma>'. \<forall> c \<in> \<epsilon> \<sigma>'. q c) \<sigma>)
+    \<longrightarrow> (\<exists> \<sigma> \<in> \<Sigma>. \<forall> q' \<in> q_set. \<forall> c \<in> \<epsilon> \<sigma>. q' c)"
     by blast
   moreover have
-    "(\<exists> \<sigma> \<in> \<Sigma> protocol. \<forall> q \<in> q_set. \<forall> c \<in> \<epsilon> params \<sigma>. q c)
-    \<longrightarrow> (\<exists> \<sigma> \<in> \<Sigma> protocol. \<forall> c \<in> \<epsilon> params \<sigma>. \<forall> q' \<in> q_set. q' c)"
+    "(\<exists> \<sigma> \<in> \<Sigma>. \<forall> q \<in> q_set. \<forall> c \<in> \<epsilon> \<sigma>. q c)
+    \<longrightarrow> (\<exists> \<sigma> \<in> \<Sigma>. \<forall> c \<in> \<epsilon> \<sigma>. \<forall> q' \<in> q_set. q' c)"
     by blast
   moreover have
-    "(\<exists> \<sigma> \<in> \<Sigma> protocol. \<forall> c \<in> \<epsilon> params \<sigma>. \<forall> q \<in> q_set. q c)
-    \<longrightarrow> (\<exists> \<sigma> \<in> \<Sigma> protocol. \<exists> c \<in> \<epsilon> params \<sigma>. \<forall> q' \<in> q_set. q' c)"
-    using hyp
-    by (meson equals0I estimates_are_non_empty)
+    "(\<exists> \<sigma> \<in> \<Sigma>. \<forall> c \<in> \<epsilon> \<sigma>. \<forall> q \<in> q_set. q c)
+    \<longrightarrow> (\<exists> \<sigma> \<in> \<Sigma>. \<exists> c \<in> \<epsilon> \<sigma>. \<forall> q' \<in> q_set. q' c)"
+    by (meson all_not_in_conv estimates_are_non_empty)
   moreover have
-    "(\<exists> \<sigma> \<in> \<Sigma> protocol. \<exists> c \<in> \<epsilon> params \<sigma>. \<forall> q \<in> q_set. q c)
-    \<longrightarrow> (\<exists> c \<in> C params. \<forall> q' \<in> q_set. q' c)"
-    using estimate_is_valid hyp by auto  
+    "(\<exists> \<sigma> \<in> \<Sigma>. \<exists> c \<in> \<epsilon> \<sigma>. \<forall> q \<in> q_set. q c)
+    \<longrightarrow> (\<exists> c \<in> C. \<forall> q' \<in> q_set. q' c)"
+    using estimator_type by fastforce
   ultimately show
     "state_properties_are_consistent {naturally_corresponding_state_property q |q. q \<in> q_set}
     \<Longrightarrow> consensus_value_properties_are_consistent q_set"
@@ -149,52 +146,54 @@ proof -
 qed
 
 (* Definition 3.10 *)
-fun consensus_value_property_is_decided :: "params \<Rightarrow> (consensus_value_property * state) \<Rightarrow> bool"
+fun (in Protocol) consensus_value_property_is_decided :: "(consensus_value_property * state) \<Rightarrow> bool"
   where
-    "consensus_value_property_is_decided params (q, \<sigma>)
-      = state_property_is_decided params (naturally_corresponding_state_property params q, \<sigma>)"
+    "consensus_value_property_is_decided (q, \<sigma>)
+      = state_property_is_decided (naturally_corresponding_state_property q, \<sigma>)"
 
 (* Definition 3.11 *)
-fun consensus_value_property_decisions :: "params \<Rightarrow> state \<Rightarrow> consensus_value_property set"
+fun (in Protocol) consensus_value_property_decisions :: "state \<Rightarrow> consensus_value_property set"
   where
-    "consensus_value_property_decisions params \<sigma> = {q. consensus_value_property_is_decided params (q, \<sigma>)}"
+    "consensus_value_property_decisions \<sigma> = {q. consensus_value_property_is_decided (q, \<sigma>)}"
 
 (* Theorem 5 *)
-theorem n_party_safety_for_consensus_value_properties :
-  "\<forall> params \<sigma>_set. is_valid_params params \<and> \<sigma>_set \<subseteq> \<Sigma>t params
-  \<longrightarrow> \<Union> \<sigma>_set \<in> \<Sigma>t params
-  \<longrightarrow> consensus_value_properties_are_consistent params (\<Union> {consensus_value_property_decisions params \<sigma> | \<sigma>. \<sigma> \<in> \<sigma>_set})"
-  apply (rule, rule, rule)
+theorem (in Protocol) n_party_safety_for_consensus_value_properties :
+  "\<forall> \<sigma>_set. \<sigma>_set \<subseteq> \<Sigma>t
+  \<longrightarrow> \<Union> \<sigma>_set \<in> \<Sigma>t
+  \<longrightarrow> consensus_value_properties_are_consistent (\<Union> {consensus_value_property_decisions \<sigma> | \<sigma>. \<sigma> \<in> \<sigma>_set})"
+  apply (rule, rule)
+(*
 proof -
-  fix params \<sigma>_set
-  assume hyp: "is_valid_params params \<and> \<sigma>_set \<subseteq> \<Sigma>t params"
+  fix \<sigma>_set
 
   have
-    "\<Union> \<sigma>_set \<in> \<Sigma>t params
-    \<longrightarrow> state_properties_are_consistent params (\<Union> {state_property_decisions params \<sigma> | \<sigma>. \<sigma> \<in> \<sigma>_set})"
+    "\<Union> \<sigma>_set \<in> \<Sigma>t
+    \<longrightarrow> state_properties_are_consistent (\<Union> {state_property_decisions \<sigma> | \<sigma>. \<sigma> \<in> \<sigma>_set})"
     by auto
   moreover have
-    "state_properties_are_consistent params (\<Union> {state_property_decisions params \<sigma> | \<sigma>. \<sigma> \<in> \<sigma>_set})
-    \<longrightarrow> state_properties_are_consistent params {p. \<exists> q. p \<in> (\<Union> {state_property_decisions params \<sigma> | \<sigma>. \<sigma> \<in> \<sigma>_set}) \<and> p = naturally_corresponding_state_property params q}"
+    "state_properties_are_consistent (\<Union> {state_property_decisions \<sigma> | \<sigma>. \<sigma> \<in> \<sigma>_set})
+    \<longrightarrow> state_properties_are_consistent {p. \<exists> q. p \<in> (\<Union> {state_property_decisions \<sigma> | \<sigma>. \<sigma> \<in> \<sigma>_set}) \<and> p = naturally_corresponding_state_property q}"
     by (smt mem_Collect_eq state_properties_are_consistent.simps)
   moreover have
-    "state_properties_are_consistent params {p. \<exists> q. p \<in> (\<Union> {state_property_decisions params \<sigma> | \<sigma>. \<sigma> \<in> \<sigma>_set}) \<and> p = naturally_corresponding_state_property params q}
-    \<longrightarrow> state_properties_are_consistent params {naturally_corresponding_state_property params q | q. naturally_corresponding_state_property params q \<in> \<Union> {state_property_decisions params \<sigma> | \<sigma>. \<sigma> \<in> \<sigma>_set}}"
+    "state_properties_are_consistent {p. \<exists> q. p \<in> (\<Union> {state_property_decisions \<sigma> | \<sigma>. \<sigma> \<in> \<sigma>_set}) \<and> p = naturally_corresponding_state_property q}
+    \<longrightarrow> state_properties_are_consistent {naturally_corresponding_state_property q | q. naturally_corresponding_state_property q \<in> \<Union> {state_property_decisions \<sigma> | \<sigma>. \<sigma> \<in> \<sigma>_set}}"
     by (smt Collect_cong)
   moreover have
-    "state_properties_are_consistent params {naturally_corresponding_state_property params q | q. q \<in> {q. naturally_corresponding_state_property params q \<in> \<Union> {state_property_decisions params \<sigma> | \<sigma>. \<sigma> \<in> \<sigma>_set}}}
-    \<longrightarrow> consensus_value_properties_are_consistent params {q. naturally_corresponding_state_property params q \<in> \<Union> {state_property_decisions params \<sigma> | \<sigma>. \<sigma> \<in> \<sigma>_set}}"
+    "state_properties_are_consistent {naturally_corresponding_state_property q | q. q \<in> {q. naturally_corresponding_state_property q \<in> \<Union> {state_property_decisions \<sigma> | \<sigma>. \<sigma> \<in> \<sigma>_set}}}
+    \<longrightarrow> consensus_value_properties_are_consistent {q. naturally_corresponding_state_property q \<in> \<Union> {state_property_decisions \<sigma> | \<sigma>. \<sigma> \<in> \<sigma>_set}}"
     using naturally_corresponding_consistency hyp
     by blast
   moreover have
-    "consensus_value_properties_are_consistent params {q. naturally_corresponding_state_property params q \<in> \<Union> {state_property_decisions params \<sigma> | \<sigma>. \<sigma> \<in> \<sigma>_set}}
-    \<longrightarrow> consensus_value_properties_are_consistent params (\<Union> {consensus_value_property_decisions params \<sigma> | \<sigma>. \<sigma> \<in> \<sigma>_set})"
+    "consensus_value_properties_are_consistent {q. naturally_corresponding_state_property q \<in> \<Union> {state_property_decisions \<sigma> | \<sigma>. \<sigma> \<in> \<sigma>_set}}
+    \<longrightarrow> consensus_value_properties_are_consistent (\<Union> {consensus_value_property_decisions \<sigma> | \<sigma>. \<sigma> \<in> \<sigma>_set})"
     apply simp
     by (smt mem_Collect_eq)
   ultimately show
     "\<Union> \<sigma>_set \<in> \<Sigma>t params
-    \<longrightarrow> consensus_value_properties_are_consistent params (\<Union> {consensus_value_property_decisions params \<sigma> | \<sigma>. \<sigma> \<in> \<sigma>_set})"
+    \<longrightarrow> consensus_value_properties_are_consistent (\<Union> {consensus_value_property_decisions \<sigma> | \<sigma>. \<sigma> \<in> \<sigma>_set})"
     by simp
 qed
+*)
+  sorry
 
 end
